Checkpoint merkle Tree.Put progress

src/program_proof/pav/merkle.v
@@ -1,8 +1,202 @@
 From Perennial.program_proof Require Import grove_prelude.
 From Goose.github_com.mit_pdos.pav Require Import merkle.
 
-From Perennial.program_proof.pav Require Import classes misc cryptoffi cryptoutil merkle_internal.
+From Perennial.program_proof.pav Require Import classes misc cryptoffi cryptoutil.
 From Perennial.program_proof Require Import std_proof.
+
+Section internal.
+Context `{!heapGS Σ}.
+
+Inductive tree : Type :=
+  (* Cut only exists for proof checking trees. *)
+  | Cut : list w8 → tree
+  | Empty : tree
+  | Leaf : list w8 → tree
+  | Interior : list tree → tree.
+
+Fixpoint has_entry (tr : tree) (id : list w8) (node : tree) : Prop :=
+  match tr with
+  | Cut _ => False
+  | Empty => id = [] ∧ tr = node
+  | Leaf val => id = [] ∧ tr = node
+  | Interior children =>
+    match id with
+    | [] => False
+    | pos :: rest =>
+      ∃ child, children !! Z.to_nat (word.unsigned pos) = Some child ∧ has_entry child rest node
+    end
+  end.
+
+(* The core invariant that defines the recursive hashing structure of merkle trees. *)
+Fixpoint is_node_hash (tr : tree) (hash : list w8) : iProp Σ :=
+  match tr with
+  | Cut hash' => ⌜hash = hash' ∧ length hash' = 32%nat⌝
+  | Empty => is_hash [W8 0] hash
+  | Leaf val => is_hash (val ++ [W8 1]) hash
+  | Interior children =>
+    ∃ (child_hashes : list (list w8)),
+    let map_fn := (λ c h, is_node_hash c h) in
+    ([∗ list] child_fn;hash' ∈ (map_fn <$> children);child_hashes,
+      child_fn hash') ∗
+    is_hash (concat child_hashes ++ [W8 2]) hash
+  end%I.
+
+#[global]
+Instance is_node_hash_timeless tr hash : Timeless (is_node_hash tr hash).
+Proof. Admitted.
+
+#[global]
+Instance is_node_hash_persistent tr hash : Persistent (is_node_hash tr hash).
+Proof. Admitted.
+
+Lemma node_hash_len tr hash :
+  is_node_hash tr hash -∗ ⌜length hash = 32%nat⌝.
+Proof.
+  iIntros "Htree".
+  destruct tr.
+  { iDestruct "Htree" as "[%Heq %Hlen]". naive_solver. }
+  1-2: iDestruct (is_hash_len with "Htree") as "%Hlen"; naive_solver.
+  {
+    iDestruct "Htree" as (ch) "[_ Htree]".
+    by iDestruct (is_hash_len with "Htree") as "%Hlen".
+  }
+Qed.
+
+Lemma concat_len_eq {A : Type} sz (l1 l2 : list (list A)) :
+  concat l1 = concat l2 →
+  (Forall (λ l, length l = sz) l1) →
+  (Forall (λ l, length l = sz) l2) →
+  0 < sz →
+  l1 = l2.
+Proof.
+  intros Heq_concat Hlen_l1 Hlen_l2 Hsz.
+  apply (f_equal length) in Heq_concat as Heq_concat_len.
+  do 2 rewrite concat_length in Heq_concat_len.
+  generalize dependent l2.
+  induction l1 as [|a1]; destruct l2 as [|a2]; simpl;
+    intros Heq_concat Hlen_l2 Heq_concat_len;
+    decompose_Forall; eauto with lia.
+  apply (f_equal (take (length a1))) in Heq_concat as Htake_concat.
+  apply (f_equal (drop (length a1))) in Heq_concat as Hdrop_concat.
+  rewrite <-H in Htake_concat at 2.
+  rewrite <-H in Hdrop_concat at 2.
+  do 2 rewrite take_app_length in Htake_concat.
+  do 2 rewrite drop_app_length in Hdrop_concat.
+  rewrite Htake_concat.
+  apply (app_inv_head_iff [a2]).
+  apply IHl1; eauto with lia.
+Qed.
+
+(* TODO: is this necessary? can we just apply node_hash_len when necessary? *)
+Lemma sep_node_hash_len ct ch :
+  ([∗ list] t;h ∈ ct;ch, is_node_hash t h) -∗
+  ⌜Forall (λ l, length l = 32%nat) ch⌝.
+Proof.
+  iIntros "Htree".
+  iDestruct (big_sepL2_impl _ (λ _ _ h, ⌜length h = 32%nat⌝%I) with "Htree []") as "Hlen_sepL2".
+  {
+    iIntros "!>" (???) "_ _ Hhash".
+    by iDestruct (node_hash_len with "Hhash") as "Hlen".
+  }
+  iDestruct (big_sepL2_const_sepL_r with "Hlen_sepL2") as "[_ %Hlen_sepL1]".
+  iPureIntro.
+  by apply Forall_lookup.
+Qed.
+
+Lemma disj_empty_leaf digest v :
+  is_node_hash Empty digest -∗
+  is_node_hash (Leaf v) digest -∗
+  False.
+Proof.
+  iIntros "Hempty Hleaf".
+  iDestruct (is_hash_inj with "Hempty Hleaf") as "%Heq".
+  iPureIntro.
+  destruct v as [|a]; [naive_solver|].
+  (* TODO: why doesn't list_simplifier or solve_length take care of this? *)
+  apply (f_equal length) in Heq.
+  rewrite length_app in Heq.
+  simpl in *.
+  lia.
+Qed.
+
+(* Ownership of a logical merkle tree. *)
+Definition own_node_except' (recur : option (list w8) -d> loc -d> tree -d> iPropO Σ) : option (list w8) -d> loc -d> tree -d> iPropO Σ :=
+  (λ path ptr_tr tr,
+    match tr with
+    (* We should never have cuts in in-memory trees. *)
+    | Cut _ => False
+    | Empty => True
+    | Leaf val =>
+      ∃ sl_val hash sl_hash,
+      "Hval" ∷ own_slice_small sl_val byteT (DfracOwn 1) val ∗
+      "Hptr_val" ∷ ptr_tr ↦[node :: "val"] (slice_val sl_val) ∗
+      "Hhash" ∷ own_slice_small sl_hash byteT (DfracOwn 1) hash ∗
+      "Hsl_hash" ∷ ptr_tr ↦[node :: "hash"] (slice_val sl_hash) ∗
+      "#His_hash" ∷ match path with
+        | None => is_node_hash tr hash
+        | _ => True
+        end
+    | Interior children =>
+      ∃ hash sl_hash sl_children ptr_children sl_val,
+      "Hhash" ∷ own_slice_small sl_hash byteT (DfracOwn 1) hash ∗
+      "Hsl_children" ∷ own_slice_small sl_children ptrT (DfracOwn 1) ptr_children ∗
+      "Hptr_val" ∷ ptr_tr ↦[node :: "val"] (slice_val sl_val) ∗  (* XXX: keeping this to ensure ptr_tr is not null *)
+      "Hptr_children" ∷ ptr_tr ↦[node :: "Children"] (slice_val sl_children) ∗
+      "Hchildren" ∷
+        ([∗ list] idx ↦ child;ptr_child ∈ children;ptr_children,
+           match path with
+           | Some (a :: path) => if decide (uint.nat a = idx) then ▷ recur (Some path) ptr_child child
+                               else ▷ recur None ptr_child child
+           | None => ▷ recur None ptr_child child
+           | Some [] => ▷ recur None ptr_child child
+           end
+        ) ∗
+      "#His_hash" ∷ match path with
+      | None => is_node_hash tr hash
+      | _ => True
+      end
+    end)%I.
+
+Local Instance own_node_except'_contractive : Contractive own_node_except'.
+Proof. Admitted.
+
+Definition own_node_except : option (list w8) → loc → tree → iProp Σ := fixpoint own_node_except'.
+
+Lemma own_node_except_unfold path ptr obj :
+  own_node_except path ptr obj ⊣⊢ (own_node_except' own_node_except) path ptr obj.
+Proof.
+  apply (fixpoint_unfold own_node_except').
+Qed.
+
+Definition tree_to_map (tr : tree) : gmap (list w8) (list w8) :=
+  let fix traverse (tr : tree) (acc : gmap (list w8) (list w8)) (id : list w8) :=
+    match tr with
+    | Cut _ => acc
+    | Empty => acc
+    | Leaf val => <[id:=val]>acc
+    | Interior children =>
+      (* Grab all entries from the children, storing the ongoing id. *)
+      (foldr
+        (λ child (pIdxAcc:(Z * gmap (list w8) (list w8))),
+          let acc' := traverse child pIdxAcc.2 (id ++ [W8 pIdxAcc.1])
+          in (pIdxAcc.1 + 1, acc'))
+        (0, acc) children
+      ).2
+    end
+  in traverse tr ∅ [].
+
+Lemma own_node_except_mono path2 path1 root tr :
+  match path1, path2 with
+  | Some a, Some b => prefix a b
+  | None, _ => True
+  | _, _ => False
+  end →
+  own_node_except path1 root tr -∗
+  own_node_except path2 root tr.
+Proof.
+Admitted.
+
+End internal.
 
 Section external.
 Context `{!heapGS Σ}.
@@ -153,7 +347,7 @@ Section local_defs.
 Context `{!heapGS Σ}.
 Definition own (ptr : loc) (obj : t) : iProp Σ :=
   ∃ sl_Val sl_Dig sl_Proof,
-  "HVal" ∷ ptr ↦[GetReply :: "Val"] (slice_val sl_Val) ∗
+  "HVal" ∷ ptr ↦[GetReply :: "val"] (slice_val sl_Val) ∗
   "Hptr_Val" ∷ own_slice_small sl_Val byteT (DfracOwn 1) obj.(Val) ∗
   "HDig" ∷ ptr ↦[GetReply :: "Digest"] (slice_val sl_Dig) ∗
   "Hptr_Dig" ∷ own_slice_small sl_Dig byteT (DfracOwn 1) obj.(Digest) ∗
@@ -201,7 +395,90 @@ Lemma wp_Tree_Put ptr_tr entries sl_id id sl_val val d0 d1 :
       else
         "Htree" ∷ own_merkle ptr_tr entries
   }}}.
-Proof. Admitted.
+Proof.
+  iIntros (?) "H HΦ". iNamed "H".
+  wp_rec.
+  wp_pures.
+  iDestruct (own_slice_small_sz with "Hid") as %Hsz_id.
+  wp_apply wp_slice_len.
+  wp_pures.
+  wp_if_destruct.
+  { (* return an error. *)
+    wp_pures.
+    replace (slice.nil) with (slice_val Slice.nil) by done.
+    iApply "HΦ".
+    iModIntro. iFrame. iPureIntro.
+    word.
+  }
+  wp_rec.
+  wp_pures.
+  iNamed "Htree".
+  wp_loadField.
+  wp_pures.
+
+  (* weaken to loop invariant. *)
+  iDestruct (own_node_except_mono (Some id) with "[$]") as "Hnode".
+  { done. }
+
+  wp_bind (if: _ then _ else _)%E.
+  wp_apply (wp_wand _ _ _ (λ _,
+                             ∃ (root : loc) tr,
+                               "Hroot" ∷ ptr_tr ↦[Tree::"root"] #root ∗
+                               "Hnode" ∷ own_node_except (Some id) root tr ∗
+                               "%Htree" ∷ ⌜ tree_to_map tr = entries ⌝
+              )%I
+             with "[Hnode Hroot]").
+  {
+    wp_if_destruct.
+    2:{ iModIntro. iFrame "∗%". }
+    wp_rec.
+    wp_apply wp_NewSlice.
+    iIntros (?) "Hsl".
+    wp_pures. wp_apply wp_allocStruct.
+    { val_ty. }
+
+    (* establish that tr = Empty *)
+    iDestruct (own_node_except_unfold with "Hnode") as "Hnode".
+    rewrite /own_node_except'.
+    destruct tr.
+    { done. }
+    2:{ iNamed "Hnode".
+        by iDestruct (struct_field_pointsto_not_null with "Hptr_val") as %Hn.
+    }
+    2:{ iNamed "Hnode".
+        by iDestruct (struct_field_pointsto_not_null with "Hptr_val") as %Hn.
+    }
+    iClear "Hnode".
+    iIntros (?) "Hnode".
+    iDestruct (struct_fields_split with "Hnode") as "Hnode".
+    iNamed "Hnode".
+    wp_storeField.
+    iFrame.
+    iExists Empty.
+    iSplitL; last done.
+    by iApply own_node_except_unfold.
+  }
+  iIntros (?) "HifInv".
+  wp_pures. clear v.
+  wp_apply wp_ref_of_zero.
+  { done. }
+  iIntros (nodePath_ptr) "HnodePath_ptr".
+  wp_pures.
+  iNamed "HifInv".
+  wp_loadField.
+  wp_load.
+  rewrite zero_slice_val.
+  wp_apply (wp_SliceAppend (V:=loc) with "[]").
+  { iApply own_slice_zero. }
+  iIntros (?) "HnodePath".
+  simpl.
+  wp_store.
+  wp_apply wp_ref_to.
+  { val_ty. }
+  iIntros (pathIdx_ptr) "HpathIdx".
+  wp_pures.
+  wp_apply (wp_forUpto' with "[$HpathIdx]").
+Admitted.
 
 Lemma wp_Tree_Get ptr_tr entries sl_id id d0 :
   {{{
